\documentclass{article}
\usepackage{amsmath}

\begin{document}\noindent

\begin{enumerate}
\item 
\begin{align*}
V_{in}(\omega, t) &= I(\omega, t)Z(\omega) \\
V_{in}(\omega, t) &= I(\omega, t)\left[ R + \frac{1}{i\omega C}\right] \\
\frac{i \omega C V_{in}(\omega, t)}{1 + i\omega C R} &= I(\omega, t) 
\end{align*}
\begin{align*}
\frac{1}{CR} &= \omega_0\\
\omega C R &= \frac{\omega}{\omega_0} = \omega'
\end{align*}
\begin{align*}
V_{out}(\omega, t) &= I(\omega, t) R \\
                  &= \frac{i\omega C R V_{in}(\omega, t)}{1 + i\omega C R} =
\frac{i\omega' V_{in}(\omega, t)}{1 + i\omega'}\\
       g e^{i \phi} &= \frac{i \omega'}{1 + i \omega'}  = \frac{\omega'}{\omega' - i}\\
       g &= \frac{\omega'}{\sqrt{1 + \omega'^2}}\\
e^{i\phi} &= \frac{1}{g}\frac{i\omega'}{1 + i\omega'} = |A| i(1 - i\omega')
= |A| (\omega' + i) \\
\phi &= \tan^{-1}(1/\omega') = \tan^{-1}(1/\omega C R)
\end{align*}

\end{enumerate}

\end{document}